theories/interop/wrapper_wp_ext_call_laws.v
@@ -151,6 +151,95 @@ Proof.
         do 2 iExists _; iFrame. done.
 Qed.
 
+Lemma wp_ext_call_registerroot : ext_call_is_sound WP_registerroot_spec.
+Proof.
+  intros E T s vv K Ξ Φ.
+  rewrite weakestpre.wp_unfold. rewrite /weakestpre.wp_pre.
+  iIntros "%Hnone Hnb HT IH %σ Hσ".
+  destruct σ as [ρml σ | ρc mem].
+  1: iExFalso; iNamed "Hσ"; iNamed "SIML"; iPoseProof (ghost_var_agree with "Hnb HAbound") as "%HH"; congruence.
+  iNamed "Hσ"; iNamed "SIC".
+  cbn. unfold WP_registerroot_spec. iNamed "HT". iNamed "HGC".
+  iPoseProof (ghost_var_agree with "HAGCθ HAθ") as "%H"; subst θ.
+
+  iAssert (⌜l ∈ dom roots_m⌝ → False)%I as "%Hdom".
+  1: { iIntros "%H". eapply elem_of_dom in H; destruct H as [k Hk].
+       iPoseProof (big_sepM_lookup_acc with "Hrootspto") as "((%ww&Hww&_)&_)".
+       1: apply Hk. iPoseProof (mapsto_ne with "Hpto Hww") as "%Hne". congruence. }
+  iPoseProof (ghost_var_agree with "HAroots HArootss") as "%Heq"; subst roots_s.
+
+  iModIntro. iRight. iRight. iSplitR.
+  + iPureIntro. econstructor. eapply head_prim_step.
+    eapply (PrimRegisterrootS _ _ _ _ _ _ _ (fun k => True)). 1,3,4: done.
+    intros H; apply Hdom; congruence.
+  + iIntros (X Hstep).
+    destruct Hstep as ([] & x & Hre & Hstep). change (fill () x) with x in Hre. subst x.
+    cbn in Hstep; unfold step,mrel in Hstep; cbn in Hstep.
+    inversion_call_step Hstep ([ #l ]). subst.
+
+    iMod (ghost_var_update_halves with "HAroots HArootss") as "(HAroots&HArootss)".
+    iMod (ghost_map_insert with "HArootsm") as "(HArootsm&Hres)". 
+    1: eapply not_elem_of_dom; intros Hc; eapply Hdom; done.
+    iPoseProof (big_sepM_insert) as "(_&HR)".
+    1: eapply not_elem_of_dom; intros Hc; eapply Hdom; done.
+    iPoseProof ("HR" with "[Hpto Hrootspto]") as "Hrootspto"; first iFrame "Hrootspto".
+    iExists w; iFrame; done.
+    iClear "HR".
+    do 3 iModIntro.
+    do 2 iExists _. change (Wrap.fill () ?x) with (x) in H6.
+    iSplitR; first (iPureIntro; eapply H6).
+    iSplitR "Hnb IH HWP HAGCθ HAGCbound HArootss HArootsm Hrootspto Hres".
+    * cbn. unfold C_state_interp. iSplitL "HσC HnC"; first (iExists nCv; iFrame).
+      repeat iExists _. iFrame. iSplitL; first by iExists _. iPureIntro; done.
+    * iApply ("IH" with "[-Hnb] Hnb").
+      iApply ("HWP" with "[-Hres] Hres").
+      iExists _, _. iFrame. iPureIntro; split_and!.
+      - rewrite dom_insert_L. rewrite Heq. done.
+      - intros ℓ γ [[-> ->]|[Hne HH]]%lookup_insert_Some; last by eapply Hrootslive.
+        inversion Hrepr; subst. by eapply elem_of_dom_2.
+Qed.
+
+Lemma wp_ext_call_unregisterroot : ext_call_is_sound WP_unregisterroot_spec.
+Proof.
+  intros E T s vv K Ξ Φ.
+  rewrite weakestpre.wp_unfold. rewrite /weakestpre.wp_pre.
+  iIntros "%Hnone Hnb HT IH %σ Hσ".
+  destruct σ as [ρml σ | ρc mem].
+  1: iExFalso; iNamed "Hσ"; iNamed "SIML"; iPoseProof (ghost_var_agree with "Hnb HAbound") as "%HH"; congruence.
+  iNamed "Hσ"; iNamed "SIC".
+  cbn. unfold WP_unregisterroot_spec. iNamed "HT". iNamed "HGC".
+  iPoseProof (ghost_var_agree with "HAGCθ HAθ") as "%H"; subst θ.
+
+  iPoseProof (ghost_map_lookup with "HArootsm Hpto") as "%Helem".
+  iPoseProof (ghost_var_agree with "HAroots HArootss") as "%Heq"; subst roots_s.
+
+  iModIntro. iRight. iRight. iSplitR.
+  + iPureIntro. econstructor. eapply head_prim_step.
+    eapply (PrimUnregisterrootS _ _ _ _ _ _ _ (fun k => True)). 1,3,4: done.
+    rewrite Heq; by eapply elem_of_dom_2.
+  + iIntros (X Hstep).
+    destruct Hstep as ([] & x & Hre & Hstep). change (fill () x) with x in Hre. subst x.
+    cbn in Hstep; unfold step,mrel in Hstep; cbn in Hstep.
+    inversion_call_step Hstep ([ #l ]). subst.
+
+    iMod (ghost_var_update_halves with "HAroots HArootss") as "(HAroots&HArootss)".
+    iMod (ghost_map_delete with "HArootsm Hpto") as "HArootsm".
+    iPoseProof (big_sepM_delete) as "(HL&_)"; first eapply Helem.
+    iPoseProof ("HL" with "Hrootspto") as "((%W&Hpto&%Hw)&Hrootspto)".
+    iClear "HL".
+    do 3 iModIntro.
+    do 2 iExists _. change (Wrap.fill () ?x) with (x) in H6.
+    iSplitR; first (iPureIntro; eapply H6).
+    iSplitR "Hnb IH HWP HAGCθ HAGCbound HArootss HArootsm Hrootspto Hpto".
+    * cbn. unfold C_state_interp. iSplitL "HσC HnC"; first (iExists nCv; iFrame).
+      repeat iExists _. iFrame. iSplitL; first by iExists _. iPureIntro; done.
+    * iApply ("IH" with "[-Hnb] Hnb").
+      iApply ("HWP" $! W with "[-Hpto] Hpto []"). 2: done.
+      iExists _, _. iFrame. iPureIntro; split_and!.
+      - rewrite dom_delete_L. rewrite Heq. done.
+      - intros ℓ γ [HH1 HH2]%lookup_delete_Some; by eapply Hrootslive.
+Qed.
+
 Ltac solve_ext_call H := 
     iPoseProof (H with "[] Hnb H [IH]") as "Hwp"; [done
     | iIntros "!> %r HΞ Hnb"; iApply ("IH" with "HΞ Hnb"); by iApply "Hr"
@@ -169,9 +258,11 @@ Proof.
   destruct σ as [ρml σ | ρc mem].
   1: iExFalso; iNamed "Hσ"; iNamed "SIML"; iPoseProof (ghost_var_agree with "Hnb HAbound") as "%HH"; congruence.
   iNamed "Hσ"; iNamed "SIC".
-  cbn. iDestruct "HT" as "[H|H]".
+  cbn. iDestruct "HT" as "[H|[H|[H|H]]]".
   - solve_ext_call wp_ext_call_int2val.
   - solve_ext_call wp_ext_call_val2int.
+  - solve_ext_call wp_ext_call_registerroot.
+  - solve_ext_call wp_ext_call_unregisterroot.
 Qed.
 
 
